theories/BisimStruct.v
@@ -363,12 +363,12 @@ Module Sanity.
       2: { apply matching_active_refl; auto. eapply scheduled_active_; eauto. }
       inv H. apply inj_pair2 in H3. subst. remember 2. destruct x; inv Heqn.
       + apply SchedChoice with (x:=Fin.FS Fin.F1); auto.
-      + apply SchedChoice with (x0:=Fin.F1); auto.
+      + apply SchedChoice with (x:=Fin.F1); auto.
     - intros. exists t'. split.
       2: { apply matching_active_refl; auto. eapply scheduled_active_; eauto. }
       inv H. apply inj_pair2 in H3. subst. remember 2. destruct x; inv Heqn.
       + apply SchedChoice with (x:=Fin.FS Fin.F1); auto.
-      + apply SchedChoice with (x0:=Fin.F1); auto.
+      + apply SchedChoice with (x:=Fin.F1); auto.
   Qed.
 
   (* To generalize to any arity *)
@@ -382,8 +382,8 @@ Module Sanity.
       inv H. apply inj_pair2 in H3. subst. remember 2. destruct x; inv Heqn.
       + inv H4. apply inj_pair2 in H2. subst. remember 2. destruct x; inv Heqn.
         * apply SchedChoice with (x:=Fin.F1); auto.
-        * apply SchedChoice with (x0:=Fin.FS Fin.F1); auto.
-      + apply SchedChoice with (x0:=Fin.FS (Fin.FS Fin.F1)); auto.
+        * apply SchedChoice with (x:=Fin.FS Fin.F1); auto.
+      + apply SchedChoice with (x:=Fin.FS (Fin.FS Fin.F1)); auto.
     - intros. exists t'. split.
       2: { apply matching_active_refl; auto. eapply scheduled_active_; eauto. }
       inv H. apply inj_pair2 in H3. subst. remember 3. destruct x; inv Heqn.
@@ -392,7 +392,7 @@ Module Sanity.
       + remember 2. destruct x; inv Heqn.
         * apply SchedChoice with (x:=Fin.F1).
           apply SchedChoice with (x:=Fin.FS Fin.F1); auto.
-        * apply SchedChoice with (x0:=Fin.FS Fin.F1); auto.
+        * apply SchedChoice with (x:=Fin.FS Fin.F1); auto.
   Qed.
 
   Lemma choice2_spinI : forall {E X} (t : ctree E X),
