theories/Trans.v
@@ -76,21 +76,21 @@ Section Trans.
 	  | obs {X : Type} (e : E X) (v : X)
 	  | val {X : Type} (v : X).
 
-    Inductive visible_ : hrel S' S' :=
-    | VisibleI {n} (x : Fin.t n) k t :
-      visible_ (observe (k x)) t ->
-      visible_ (ChoiceF false n k) t
+  Inductive visible_ : hrel S' S' :=
+  | VisibleI {n} (x : Fin.t n) k t :
+    visible_ (observe (k x)) t ->
+    visible_ (ChoiceF false n k) t
 
-    | VisibleV {n} (x : Fin.t n) k :
-      visible_ (ChoiceF true n k) (ChoiceF true n k)
+  | VisibleV {n} (x : Fin.t n) k :
+    visible_ (ChoiceF true n k) (ChoiceF true n k)
 
-    | VisibleVis {X} (e : E X) k :
-      visible_ (VisF e k) (VisF e k)
+  | VisibleVis {X} (e : E X) k :
+    visible_ (VisF e k) (VisF e k)
 
 	| VisibleRet r :
-      visible_ (RetF r) (RetF r)
-    .
-    Hint Constructors visible_ : core.
+    visible_ (RetF r) (RetF r)
+  .
+  Hint Constructors visible_ : core.
 
 	Definition visibleR : hrel S S :=
 	  fun u v => visible_ (observe u) (observe v).
@@ -99,7 +99,7 @@ Section Trans.
 		Proper (equ eq ==> equ eq ==> iff) visibleR.
 	Proof.
 		intros ? ? eqt ? ? equ; unfold visibleR.
-        Admitted.
+  Admitted.
 
 	Definition visible : srel SS SS := {| hrel_of := visibleR : hrel SS SS |}.
 
